\problem

\subproblem
\[ P(1'5 < x \leq 2) = \int_{1'5}^{2} f(x) \,dx  = \int_{1'5}^{2} \frac{2x-1}{10} \,dx = \frac{1}{10}[\int 2x \,dx - \int \,dx] = \frac{2}{10} - 0'075 = 0'125\] 
\[P(2'5<x\leq 3'5) = 0\] 
\[P(4'5<x\leq5'5) = \int_{4'5}^{5'5} 0'4 \,dx = 2'2 - 1'8 = 0'4 \]
\[P(1'2 < x \leq 5'2) = \int_{1'2}^2 \frac{2x-1}{10} \,dx + \int_4^{5'2} 0'4 \,dx = 0'2 - 0'024 + 2'08 - 1'6 = 0'656\] \\ \\
\subproblem
\[E[X] = \int_{-\infty}^\infty x*f(x) \,dx = \int_1^2 \frac{2x-1}{10}*x \,dx + \int_4^6 0'4x \,dx = \frac{259}{60} \simeq 4'317 \] 
\[ M_k = \int_{-\infty}^\infty x^k * f(x) \,dx = \int_1^2 \frac{2x-1}{10}* x^k \,dx + \int_4^6 0'4*x^k \,dx \]
\subproblem
\[M_x(t) = E(e^{xt}) = \int_{-\infty}^{\infty} e^{xt} * f(x) \,dx = \int_1^2 \frac{2x-1}{10}*e^{xt} \,dx + \int_4^6 0'4 * e^{xt} \,dx = \] \[ \frac{e^t((3t-2)e^t-t+2)}{10t^2}+ \frac{2(e^{2t}-1)e^{4t}}{5t}\]
